Runwai/Eval.lean
@@ -66,93 +66,138 @@ def evalBoolOp (op : BooleanOp) : Value → Value → Option Bool
     | BooleanOp.or  => x || y
   | _, _ => none
 
-mutual
-  inductive EvalProp : ValEnv → ChipEnv → Expr → Value → Prop
-    -- E‑VALUE
-    | ConstF        {σ Δ v} : EvalProp σ Δ (Expr.constF v) (Value.vF v)
-    | ConstZ        {σ Δ v} : EvalProp σ Δ (Expr.constZ v) (Value.vZ v)
-    | ConstBool     {σ Δ b} : EvalProp σ Δ (Expr.constBool b) (Value.vBool b)
-    | ConstArr  {σ Δ xs es} (ilength: xs.length = es.length) (ih : ∀ xe ∈ List.zip xs es, EvalProp σ Δ xe.fst xe.snd) :
-        EvalProp σ Δ (Expr.arr xs) (Value.vArr es)
+inductive EvalProp : ValEnv → TraceEnv → ChipEnv → Expr → Value → Prop
+  -- E‑VALUE
+  | ConstF        {σ T Δ v} : EvalProp σ T Δ (Expr.constF v) (Value.vF v)
+  | ConstZ        {σ T Δ v} : EvalProp σ T Δ (Expr.constZ v) (Value.vZ v)
+  | ConstBool     {σ T Δ b} : EvalProp σ T Δ (Expr.constBool b) (Value.vBool b)
+  | ConstArr  {σ T Δ xs es} (ilength: xs.length = es.length) (ih : ∀ xe ∈ List.zip xs es, EvalProp σ T Δ xe.fst xe.snd) :
+      EvalProp σ T Δ (Expr.arr xs) (Value.vArr es)
 
-    | toZ {σ Δ e v} (h: EvalProp σ Δ e (Ast.Value.vF v)) :
-        EvalProp σ Δ (Expr.toZ e) (Ast.Value.vZ v.val)
+  | toZ {σ T Δ e v} (h: EvalProp σ T Δ e (Ast.Value.vF v)) :
+      EvalProp σ T Δ (Expr.toZ e) (Ast.Value.vZ v.val)
 
-    -- E‑VAR
-    | Var         {σ Δ x v} : lookupVal σ x = v → EvalProp σ Δ (Expr.var x) v
+  -- E‑VAR
+  | Var {σ T Δ x v} : lookupVal σ x = v → EvalProp σ T Δ (Expr.var x) v
 
-    -- E‑LAM
-    | Lam    {σ Δ x τ body} : EvalProp σ Δ (Expr.lam x τ body) (Value.vClosure x body σ)
+  -- E‑LAM
+  | Lam {σ T Δ x τ body} : EvalProp σ T Δ (Expr.lam x τ body) (Value.vClosure x body σ)
 
-    -- E‑LET
-    | Let      {σ Δ x e₁ e₂ v₁ v₂}
-        (ih₁ : EvalProp σ Δ e₁ v₁)
-        (ih₂ : EvalProp (updateVal σ x v₁) Δ e₂ v₂) :
-        EvalProp σ Δ (Expr.letIn x e₁ e₂) v₂
+  -- E‑LET
+  | Let      {σ T Δ x e₁ e₂ v₁ v₂}
+      (ih₁ : EvalProp σ T Δ e₁ v₁)
+      (ih₂ : EvalProp (updateVal σ x v₁) T Δ e₂ v₂) :
+      EvalProp σ T Δ (Expr.letIn x e₁ e₂) v₂
 
-    -- E‑APP
-    | App      {σ Δ f a x body σ' va vb}
-        (ih_f : EvalProp σ Δ f (Value.vClosure x body σ'))
-        (ih_a : EvalProp σ Δ a va)
-        (ih_b : EvalProp (updateVal σ' x va) Δ body vb) :
-        EvalProp σ Δ (Expr.app f a) vb
+  -- E‑APP
+  | App      {σ T Δ f a x body σ' va vb}
+      (ih_f : EvalProp σ T Δ f (Value.vClosure x body σ'))
+      (ih_a : EvalProp σ T Δ a va)
+      (ih_b : EvalProp (updateVal σ' x va) T Δ body vb) :
+      EvalProp σ T Δ (Expr.app f a) vb
 
-    -- E‑FBINOP
-    | FBinOp   {σ Δ e₁ e₂ op i₁ i₂ v}
-        (ih₁ : EvalProp σ Δ e₁ (Value.vF i₁))
-        (ih₂ : EvalProp σ Δ e₂ (Value.vF i₂))
-        (r   : evalFieldOp op (Value.vF i₁) (Value.vF i₂) = some v) :
-        EvalProp σ Δ (Expr.fieldExpr e₁ op e₂) v
+  -- E‑FBINOP
+  | FBinOp   {σ T Δ e₁ e₂ op i₁ i₂ v}
+      (ih₁ : EvalProp σ T Δ e₁ (Value.vF i₁))
+      (ih₂ : EvalProp σ T Δ e₂ (Value.vF i₂))
+      (r   : evalFieldOp op (Value.vF i₁) (Value.vF i₂) = some v) :
+      EvalProp σ T Δ (Expr.fieldExpr e₁ op e₂) v
 
-    -- E‑ZBINOP
-    | ZBinOp   {σ Δ e₁ e₂ op i₁ i₂ v}
-        (ih₁ : EvalProp σ Δ e₁ (Value.vZ i₁))
-        (ih₂ : EvalProp σ Δ e₂ (Value.vZ i₂))
-        (r   : evalIntegerOp op (Value.vZ i₁) (Value.vZ i₂) = some v) :
-        EvalProp σ Δ (Expr.integerExpr e₁ op e₂) v
+  -- E‑ZBINOP
+  | ZBinOp   {σ T Δ e₁ e₂ op i₁ i₂ v}
+      (ih₁ : EvalProp σ T Δ e₁ (Value.vZ i₁))
+      (ih₂ : EvalProp σ T Δ e₂ (Value.vZ i₂))
+      (r   : evalIntegerOp op (Value.vZ i₁) (Value.vZ i₂) = some v) :
+      EvalProp σ T Δ (Expr.integerExpr e₁ op e₂) v
 
-    -- E‑BOOLBINOP
-    | BoolOp   {σ Δ e₁ e₂ op b₁ b₂ b}
-        (ih₁ : EvalProp σ Δ e₁ (Value.vBool b₁))
-        (ih₂ : EvalProp σ Δ e₂ (Value.vBool b₂))
-        (bv  : evalBoolOp op (Value.vBool b₁) (Value.vBool b₂) = some b) :
-        EvalProp σ Δ (Expr.boolExpr e₁ op e₂) (Value.vBool b)
+  -- E‑BOOLBINOP
+  | BoolOp   {σ T Δ e₁ e₂ op b₁ b₂ b}
+      (ih₁ : EvalProp σ T Δ e₁ (Value.vBool b₁))
+      (ih₂ : EvalProp σ T Δ e₂ (Value.vBool b₂))
+      (bv  : evalBoolOp op (Value.vBool b₁) (Value.vBool b₂) = some b) :
+      EvalProp σ T Δ (Expr.boolExpr e₁ op e₂) (Value.vBool b)
 
-    -- E‑REL
-    | Rel      {σ Δ e₁ e₂ op v₁ v₂ b}
-        (ih₁ : EvalProp σ Δ e₁ v₁)
-        (ih₂ : EvalProp σ Δ e₂ v₂)
-        (r   : evalRelOp op v₁ v₂ = some b) :
-        EvalProp σ Δ (Expr.binRel e₁ op e₂) (Value.vBool b)
+  -- E‑REL
+  | Rel      {σ T Δ e₁ e₂ op v₁ v₂ b}
+      (ih₁ : EvalProp σ T Δ e₁ v₁)
+      (ih₂ : EvalProp σ T Δ e₂ v₂)
+      (r   : evalRelOp op v₁ v₂ = some b) :
+      EvalProp σ T Δ (Expr.binRel e₁ op e₂) (Value.vBool b)
 
-    -- E-BRANCH
-    | IfTrue {σ Δ c e₁ e₂ v₁}
-        (ihc : EvalProp σ Δ c (Value.vBool true))
-        (ih₁ : EvalProp σ Δ e₁ v₁):
-        EvalProp σ Δ (Expr.branch c e₁ e₂) (v₁)
+  -- E-BRANCH
+  | IfTrue {σ T Δ c e₁ e₂ v₁}
+      (ihc : EvalProp σ T Δ c (Value.vBool true))
+      (ih₁ : EvalProp σ T Δ e₁ v₁):
+      EvalProp σ T Δ (Expr.branch c e₁ e₂) (v₁)
 
-    | IfFalse {σ Δ c e₁ e₂ v₂}
-        (ihc : EvalProp σ Δ c (Value.vBool false))
-        (ih₁ : EvalProp σ Δ e₂ v₂):
-        EvalProp σ Δ (Expr.branch c e₁ e₂) (v₂)
+  | IfFalse {σ T Δ c e₁ e₂ v₂}
+      (ihc : EvalProp σ T Δ c (Value.vBool false))
+      (ih₁ : EvalProp σ T Δ e₂ v₂):
+      EvalProp σ T Δ (Expr.branch c e₁ e₂) (v₂)
 
-    -- E‑ASSERT
-    | Assert   {σ Δ e₁ e₂ v}
-        (ih₁ : EvalProp σ Δ e₁ (Ast.Value.vF v))
-        (ih₂ : EvalProp σ Δ e₂ (Ast.Value.vF v)) :
-        EvalProp σ Δ (Expr.assertE e₁ e₂) (Value.vUnit)
+  -- E‑ASSERT
+  | Assert   {σ T Δ e₁ e₂ v}
+      (ih₁ : EvalProp σ T Δ e₁ (Ast.Value.vF v))
+      (ih₂ : EvalProp σ T Δ e₂ (Ast.Value.vF v)) :
+      EvalProp σ T Δ (Expr.assertE e₁ e₂) (Value.vUnit)
 
-    -- E‑ARRIDX
-    | ArrIdx {σ Δ a i vs j v}
-        (iha : EvalProp σ Δ a (Value.vArr vs))
-        (ihi : EvalProp σ Δ i (Value.vZ j))
-        (idx : vs[j]? = some v) :
-        EvalProp σ Δ (Expr.arrIdx a i) v
+  -- E‑ARRIDX
+  | ArrIdx {σ T Δ a i vs j v}
+      (iha : EvalProp σ T Δ a (Value.vArr vs))
+      (ihi : EvalProp σ T Δ i (Value.vZ j))
+      (idx : vs[j]? = some v) :
+      EvalProp σ T Δ (Expr.arrIdx a i) v
 
-    -- E-LOOKUP
-    | LookUp {σ Δ vname cname args e v}
-      (ih₁: EvalProp σ Δ e v):
-      EvalProp σ Δ (Expr.lookup vname cname args e) v
-end
+  -- E-LOOKUP
+  | LookUp {σ T Δ vname cname args e v c rows}
+    -- This constructor defines the semantics for a lookup expression, which serves a dual purpose:
+    -- 1. It enforces a set of constraints (a "lookup argument") between the calling context
+    --    and a callee chip's execution trace.
+    -- 2. It provides `let-in`-like scoping, where a subsequent expression `e` is evaluated
+    --    after the lookup constraints are satisfied.
+
+    -- == Body Evaluation Semantics ==
+    -- Premise for the `let-in` behavior. After all lookup constraints pass, this ensures
+    -- that the body expression `e` evaluates to the final value `v` of the whole expression.
+    (h_body: EvalProp σ T Δ e v)
+
+    -- == Context Setup ==
+    -- Premise to retrieve the callee's chip definition `c` from the global chip environment `Δ`.
+    (h_chip: Env.lookupChip Δ cname = c)
+    -- Premise to retrieve the callee's full execution trace `rows` from the global trace environment `T`.
+    (h_trace: Env.lookupTrace T c = some (Ast.Value.vArr (rows)))
+
+    -- == Verification of Callee's Trace ==
+    -- Premise ensuring the internal consistency of the callee's trace. It guarantees that we
+    -- are looking up into a well-formed "table" by checking that the callee's constraint body
+    -- (`c.body`) holds for ALL rows `j` of its trace.
+    (h_callee_validity:
+      ∀ j: ℕ, (j < rows.length) →
+        let σ' := Env.updateVal (Env.updateVal σ c.ident_t (Value.vArr rows)) c.ident_i (Value.vZ j)
+        EvalProp σ' T Δ c.body Value.vUnit
+    )
+
+    -- == Witnesses provided by the Prover ==
+    (i: ℕ)
+    (vs: List F)
+
+    -- == Verification of Witnesses and Lookup Connection ==
+    -- Premise checking that the witness row index `i` is within the bounds of the callee's trace.
+    (h_bound: i < rows.length)
+    -- Premise ensuring the argument list and the witness value list have the same length.
+    (h_args_len: args.length = vs.length)
+    -- Premise verifying the witness values `vs`. It proves that the caller-side expressions
+    -- (`args.map Prod.fst`) indeed evaluate to the claimed values in `vs`.
+    (h_evals:∀ p ∈ List.zip (args.map Prod.fst) vs,
+        EvalProp σ T Δ p.fst (Value.vF p.snd))
+    -- The central lookup premise. It verifies the connection between the caller and callee.
+    -- Using the witness row `i` and the verified witness values `vs`, it checks that for each
+    -- value-expression pair, the assertion holds in the callee's context at row `i`.
+    (h_asserts:
+      let σ' := Env.updateVal (Env.updateVal σ c.ident_t (Value.vArr rows)) c.ident_i (Value.vZ i)
+      ∀ p ∈ List.zip vs (args.map Prod.snd),
+        EvalProp σ' T Δ (Expr.assertE (Expr.constF p.fst) p.snd) Value.vUnit
+    )
+    :EvalProp σ T Δ (Expr.lookup vname cname args e) v
 
 end Eval
