Runwai/Gadget/TypingLemmas.lean
@@ -7,8 +7,8 @@ open Ast
 If a variable `x` is typed with a refinement `{_ : unit | e}` in a semantically valid
 environment, this lemma provides a proof that the expression `e` will evaluate to `true`.
 -/
-lemma tyenv_to_eval_expr {σ Δ Γ x τ e} (h₁: PropSemantics.tyenvToProp σ Δ Γ) (h₂: Env.lookupTy Γ x = some (Ast.Ty.refin τ (Ast.Predicate.ind e))):
-  (Eval.EvalProp σ Δ e (Ast.Value.vBool true)) := by {
+lemma tyenv_to_eval_expr {σ T Δ Γ x τ e} (h₁: PropSemantics.tyenvToProp σ T Δ Γ) (h₂: Env.lookupTy Γ x = some (Ast.Ty.refin τ (Ast.Predicate.ind e))):
+  (Eval.EvalProp σ T Δ e (Ast.Value.vBool true)) := by {
     unfold PropSemantics.tyenvToProp at h₁
     simp [PropSemantics.varToProp] at h₁
     have h₁' := h₁ x (Ast.Ty.refin τ (Ast.Predicate.ind e)) h₂
@@ -18,8 +18,8 @@ lemma tyenv_to_eval_expr {σ Δ Γ x τ e} (h₁: PropSemantics.tyenvToProp σ �
   }
 
 --  | Ast.Predicate.dep ident body => fun v => exprToProp σ Δ (Ast.Expr.app (Ast.Expr.lam ident τ body) v)
-lemma tyenv_dep_to_eval_expr {σ Δ Γ x τ body} (h₁: PropSemantics.tyenvToProp σ Δ Γ) (h₂: Env.lookupTy Γ x = some (Ast.Ty.refin τ (Ast.Predicate.dep v body))):
-  (Eval.EvalProp σ Δ (Ast.Expr.app (Ast.Expr.lam v τ body) (Ast.Expr.var x)) (Ast.Value.vBool true)) := by {
+lemma tyenv_dep_to_eval_expr {σ T Δ Γ x τ body} (h₁: PropSemantics.tyenvToProp σ T Δ Γ) (h₂: Env.lookupTy Γ x = some (Ast.Ty.refin τ (Ast.Predicate.dep v body))):
+  (Eval.EvalProp σ T Δ (Ast.Expr.app (Ast.Expr.lam v τ body) (Ast.Expr.var x)) (Ast.Value.vBool true)) := by {
     unfold PropSemantics.tyenvToProp at h₁
     simp [PropSemantics.varToProp] at h₁
     have h₁' := h₁ x (Ast.Ty.refin τ (Ast.Predicate.dep v body)) h₂
@@ -34,8 +34,8 @@ Deconstructs a **conjunctive type guarantee** into individual runtime proofs.
 If a variable's type guarantees that `e₁ ∧ e₂` holds, this lemma allows us to derive
 separate evaluation proofs for both `e₁` and `e₂`.
 -/
-lemma tyenv_and_to_eval_exprs {σ Δ Γ x e₁ e₂} (h₁: PropSemantics.tyenvToProp σ Δ Γ) (h₂: Env.lookupTy Γ x = some (Ast.Ty.refin Ast.Ty.unit (Ast.Predicate.and (Ast.Predicate.ind e₁) (Ast.Predicate.ind e₂)))):
-  (Eval.EvalProp σ Δ e₁ (Ast.Value.vBool true)) ∧ (Eval.EvalProp σ Δ e₂ (Ast.Value.vBool true)) := by {
+lemma tyenv_and_to_eval_exprs {σ T Δ Γ x e₁ e₂} (h₁: PropSemantics.tyenvToProp σ T Δ Γ) (h₂: Env.lookupTy Γ x = some (Ast.Ty.refin Ast.Ty.unit (Ast.Predicate.and (Ast.Predicate.ind e₁) (Ast.Predicate.ind e₂)))):
+  (Eval.EvalProp σ T Δ e₁ (Ast.Value.vBool true)) ∧ (Eval.EvalProp σ T Δ e₂ (Ast.Value.vBool true)) := by {
     unfold PropSemantics.tyenvToProp at h₁
     simp [PropSemantics.varToProp] at h₁
     have h₁' := h₁ x (Ast.Ty.refin Ast.Ty.unit (Ast.Predicate.and (Ast.Predicate.ind e₁) (Ast.Predicate.ind e₂))) h₂
@@ -45,22 +45,22 @@ lemma tyenv_and_to_eval_exprs {σ Δ Γ x e₁ e₂} (h₁: PropSemantics.tyenvT
   }
 
 lemma tyenvToProp_implies_varToProp
-  (σ : Env.ValEnv) (Δ : Env.ChipEnv) (Γ : Env.TyEnv)
+  (σ : Env.ValEnv) (T: Env.TraceEnv) (Δ : Env.ChipEnv) (Γ : Env.TyEnv)
   (x : String) (τ : Ast.Ty) (φ : Ast.Predicate)
   (hΓx : Env.lookupTy Γ x = Ast.Ty.refin τ φ)
-  (hmt : PropSemantics.tyenvToProp σ Δ Γ) :
-  PropSemantics.varToProp σ Δ Γ x := by
+  (hmt : PropSemantics.tyenvToProp σ T Δ Γ) :
+  PropSemantics.varToProp σ T Δ Γ x := by
   dsimp [PropSemantics.tyenvToProp] at hmt
   apply hmt
   exact hΓx
 
-lemma constZ_refine_lt {Δ Γ Η x y} {h: x < y} :
+lemma constZ_refine_lt {Δ Η x y} {h: x < y} :
   @Ty.TypeJudgment Δ Γ Η (Ast.Expr.constZ x) (Ast.Ty.int.refin (Ast.Predicate.dep Ast.mu ((Ast.Expr.var Ast.mu).binRel Ast.RelOp.lt (Ast.Expr.constZ y)))) := by {
   apply Ty.TypeJudgment.TE_SUB
   apply Ty.TypeJudgment.TE_ConstZ
   apply Ty.SubtypeJudgment.TSub_Refine
   apply Ty.SubtypeJudgment.TSub_Refl
-  intro σ v h₁ h₂
+  intro σ T v h₁ h₂
   simp [PropSemantics.predToProp] at h₂ ⊢
   cases h₂
   rename_i va ih₁ ih₂ ih₃
